Preparing to do a little more on Unification

02Typed/Type.thy
@@ -7,17 +7,28 @@ datatype ty =
   | Base 
   | Arrow ty ty
 
-primrec tsubst_var :: "var \<Rightarrow> var \<Rightarrow> ty \<Rightarrow> ty" where
-  "tsubst_var x x' (TyVar y) = TyVar (if x = y then x' else y)"
-| "tsubst_var x x' Base = Base"
-| "tsubst_var x x' (Arrow t\<^sub>1 t\<^sub>2) = Arrow (tsubst_var x x' t\<^sub>1) (tsubst_var x x' t\<^sub>2)"
-
-lemma [simp]: "size (tsubst_var x x' t) = size t"
-  by (induction t) simp_all
+primrec tvars :: "ty \<Rightarrow> var set" where
+  "tvars (TyVar y) = {y}"
+| "tvars Base = {}"
+| "tvars (Arrow t\<^sub>1 t\<^sub>2) = tvars t\<^sub>1 \<union> tvars t\<^sub>2"
 
 fun tsubst :: "var \<Rightarrow> ty \<Rightarrow> ty \<Rightarrow> ty" where
   "tsubst x t' (TyVar y) = (if x = y then t' else TyVar y)"
 | "tsubst x t' Base = Base"
 | "tsubst x t' (Arrow t\<^sub>1 t\<^sub>2) = Arrow (tsubst x t' t\<^sub>1) (tsubst x t' t\<^sub>2)"
+
+lemma [simp]: "x \<notin> tvars t \<Longrightarrow> tsubst x t' t = t"
+  by (induction t) simp_all
+
+lemma [simp]: "tsubst x (TyVar x) t = t"
+  by (induction t) simp_all
+
+lemma [simp]: "y \<notin> tvars t \<Longrightarrow> tsubst y t' (tsubst x (TyVar y) t) = tsubst x t' t"
+  by (induction t) simp_all
+
+lemma tsubst_arrow [consumes 1, case_names TyVar Arrow]: "Arrow t\<^sub>1 t\<^sub>2 = tsubst y t' tt \<Longrightarrow> 
+  (t' = Arrow t\<^sub>1 t\<^sub>2 \<Longrightarrow> tt = TyVar y \<Longrightarrow> P) \<Longrightarrow> 
+    (\<And>tt\<^sub>1 tt\<^sub>2. t\<^sub>1 = tsubst y t' tt\<^sub>1 \<Longrightarrow> t\<^sub>2 = tsubst y t' tt\<^sub>2 \<Longrightarrow> tt = Arrow tt\<^sub>1 tt\<^sub>2 \<Longrightarrow> P) \<Longrightarrow> P"
+  by (induction tt) (simp_all split: if_splits)
 
 end
