02Typed/Typechecking.thy
@@ -21,25 +21,21 @@ primrec erase :: "texpr \<Rightarrow> nexpr" where
 | "erase (TApp e\<^sub>1 e\<^sub>2) = NApp (erase e\<^sub>1) (erase e\<^sub>2)"
 
 primrec typecheck' :: "subst \<Rightarrow> var set \<Rightarrow> nexpr \<rightharpoonup> 
-    hexpr \<times> uexpr \<times> var set \<times> (var \<rightharpoonup> uexpr)" where
+    hexpr \<times> uexpr \<times> var set \<times> (uexpr \<times> uexpr) list " where
   "typecheck' \<Gamma> vs (NVar x) = (case \<Gamma> x of 
-      Some t \<Rightarrow> Some (HVar x, t, vs, \<Gamma>) 
+      Some t \<Rightarrow> Some (HVar x, t, vs, []) 
     | None \<Rightarrow> None)"
-| "typecheck' \<Gamma> vs (NConst k) = Some (HConst k, Ctor ''Base'' [], vs, \<Gamma>)"
+| "typecheck' \<Gamma> vs (NConst k) = Some (HConst k, Ctor ''Base'' [], vs, [])"
 | "typecheck' \<Gamma> vs (NLam x e) = (
     let v = fresh vs
     in case typecheck' (\<Gamma>(x \<mapsto> Var v)) (insert v vs) e of
-        Some (e', t, vs', \<Gamma>') \<Rightarrow> (case \<Gamma>' x of 
-          Some t' \<Rightarrow> Some (HLam x t' e', Ctor ''Arrow'' [t', t], vs', (\<Gamma>'(x := \<Gamma> x)))
-        | None \<Rightarrow> None)
+        Some (e', t, vs', uni) \<Rightarrow> 
+          Some (HLam x (Var v) e', Ctor ''Arrow'' [Var v, t], vs', uni)
       | None \<Rightarrow> None)"
 | "typecheck' \<Gamma> vs (NApp e\<^sub>1 e\<^sub>2) = (case typecheck' \<Gamma> vs e\<^sub>1 of
-      Some (e\<^sub>1', Ctor k [t\<^sub>1, t\<^sub>2], vs', \<Gamma>') \<Rightarrow> (
-        if k = ''Arrow'' then case typecheck' \<Gamma>' vs' e\<^sub>2 of
-            Some (e\<^sub>2', t\<^sub>3, vs'', \<Gamma>'') \<Rightarrow> (case unify t\<^sub>1 t\<^sub>2 of     
-              Some sub \<Rightarrow> Some (HApp (hsubst sub e\<^sub>1') (hsubst sub e\<^sub>2'), subst sub t\<^sub>2, vs'', 
-                                map_option (subst sub) \<circ> \<Gamma>'')
-            | None \<Rightarrow> None)
+      Some (e\<^sub>1', Ctor k [t\<^sub>1, t\<^sub>2], vs', uni\<^sub>1) \<Rightarrow> (
+        if k = ''Arrow'' then case typecheck' \<Gamma> vs' e\<^sub>2 of
+            Some (e\<^sub>2', t\<^sub>3, vs'', uni\<^sub>2) \<Rightarrow> Some (HApp e\<^sub>1' e\<^sub>2', t\<^sub>2, vs'', (t\<^sub>1, t\<^sub>3) # uni\<^sub>1 @ uni\<^sub>2)
           | None \<Rightarrow> None
         else None)
     | _ \<Rightarrow> None)"
@@ -57,6 +53,9 @@ fun valid_ty_uexpr :: "uexpr \<Rightarrow> bool" where
 | "valid_ty_uexpr (Ctor k [t\<^sub>1, t\<^sub>2]) = (k = ''Arrow'' \<and> valid_ty_uexpr t\<^sub>1 \<and> valid_ty_uexpr t\<^sub>2)"
 | "valid_ty_uexpr (Ctor k ts) = False"
 
+definition valid_ty_uexprs :: "(uexpr \<times> uexpr) list \<Rightarrow> bool" where
+  "valid_ty_uexprs ts = list_all (\<lambda>(t\<^sub>1, t\<^sub>2). valid_ty_uexpr t\<^sub>1 \<and> valid_ty_uexpr t\<^sub>2) ts"
+ 
 definition valid_ty_subst :: "subst \<Rightarrow> bool" where
   "valid_ty_subst \<Gamma> = (\<forall>t \<in> ran \<Gamma>. valid_ty_uexpr t)"
 
@@ -74,7 +73,9 @@ primrec valid_ty_hexpr :: "hexpr \<Rightarrow> bool" where
 
 fun typecheck :: "nexpr \<rightharpoonup> texpr \<times> ty" where
   "typecheck e = (case typecheck' Map.empty {} e of
-      Some (e', t, vs, \<Gamma>) \<Rightarrow> Some (solidify e', typeify t)
+      Some (e', t, vs, uni) \<Rightarrow> (case unify' uni of 
+          Some sub \<Rightarrow> Some (solidify (hsubst sub e'), typeify (subst sub t))
+        | None \<Rightarrow> None)
     | None \<Rightarrow> None)"
 
 fun tsubsts :: "subst \<Rightarrow> ty \<Rightarrow> ty" where
@@ -125,9 +126,34 @@ lemma [simp]: "valid_ty_subst \<Gamma> \<Longrightarrow> valid_ty_subst sub \<Lo
 lemma [elim]: "valid_ty_subst \<Gamma> \<Longrightarrow> \<Gamma> x = Some t \<Longrightarrow> valid_ty_uexpr t"
   by (auto simp add: valid_ty_subst_def ran_def)
 
+lemma [elim]: "valid_ty_uexpr (Ctor k es) \<Longrightarrow> list_all valid_ty_uexpr es"
+  by (induction "Ctor k es" rule: valid_ty_uexpr.induct) auto
+
+lemma [elim]: "valid_ty_uexprs ts \<Longrightarrow> unify' ts = Some sub \<Longrightarrow> valid_ty_subst sub"                                  
+proof (induction ts arbitrary: sub rule: unify'.induct)
+  case (2 k\<^sub>1 es\<^sub>1 k\<^sub>2 es\<^sub>2 ess)
+  moreover hence "list_all valid_ty_uexpr es\<^sub>1" by (auto simp add: valid_ty_uexprs_def)
+  moreover from 2 have "list_all valid_ty_uexpr es\<^sub>2" by (auto simp add: valid_ty_uexprs_def)
+  ultimately show ?case by (simp add: valid_ty_uexprs_def split: if_splits)
+next
+  case (4 x e ess)
+  from 4 have "e = Var x \<Longrightarrow> valid_ty_uexprs ess \<Longrightarrow> unify' ess = Some xsub \<Longrightarrow> valid_ty_subst xsub" by simp
+  from 4 have "e \<noteq> Var x \<Longrightarrow>
+    x \<notin> vars e \<Longrightarrow> valid_ty_uexprs (list_subst x e ess) \<Longrightarrow> unify' (list_subst x e ess) = Some xsub \<Longrightarrow> valid_ty_subst xsub" by simp
+  from 4 have "valid_ty_uexprs ((Var x, e) # ess)" by simp
+  from 4 have "unify' ((Var x, e) # ess) = Some sub" by simp
+
+  then show ?case by (auto simp add: valid_ty_uexprs_def split: if_splits)
+qed (auto simp add: valid_ty_uexprs_def)
+
 lemma [elim]: "valid_ty_uexpr t\<^sub>1 \<Longrightarrow> valid_ty_uexpr t\<^sub>2 \<Longrightarrow> unify t\<^sub>1 t\<^sub>2 = Some sub \<Longrightarrow> 
-    valid_ty_subst sub"                                  
-  by (auto simp add: valid_ty_subst_def)
+  valid_ty_subst sub"                                  
+proof (unfold unify_def)
+  assume "valid_ty_uexpr t\<^sub>1" and "valid_ty_uexpr t\<^sub>2" 
+  hence "valid_ty_uexprs [(t\<^sub>1, t\<^sub>2)]" by (simp add: valid_ty_uexprs_def)
+  moreover assume "unify' [(t\<^sub>1, t\<^sub>2)] = Some sub"
+  ultimately show "valid_ty_subst sub" by auto
+qed
 
 lemma [simp]: "valid_ty_subst sub \<Longrightarrow> valid_ty_hexpr e \<Longrightarrow> valid_ty_hexpr (hsubst sub e)"
   by (induction e) simp_all
@@ -142,121 +168,115 @@ proof (induction \<Gamma> e t rule: typecheckn.induct)
   thus ?case by blast
 qed simp_all
 
-lemma [simp]: "typecheck' \<Gamma> vs e = Some (e', t, vs', \<Gamma>') \<Longrightarrow> dom \<Gamma>' = dom \<Gamma>"
-proof (induction e arbitrary: \<Gamma> vs e' t vs' \<Gamma>')
+lemma [simp]: "valid_ty_subst \<Gamma> \<Longrightarrow> typecheck' \<Gamma> vs e = Some (e', t, vs', uni) \<Longrightarrow> 
+  valid_ty_hexpr e' \<and> valid_ty_uexpr t"
+proof (induction e arbitrary: \<Gamma> vs e' t vs' uni)
   case (NLam x e)
   let ?v = "fresh vs"
-  from NLam obtain ee' tt g\<Gamma>' t' where T: "g\<Gamma>' x = Some t' \<and> e' = HLam x t' ee' \<and> 
-    t = Ctor ''Arrow'' [t', tt] \<and> \<Gamma>' = (g\<Gamma>'(x := \<Gamma> x)) \<and>
-      typecheck' (\<Gamma>(x \<mapsto> Var ?v)) (insert ?v vs) e = Some (ee', tt, vs', g\<Gamma>')" 
-        by (auto simp add: Let_def split: option.splits)
-  with NLam have "dom g\<Gamma>' = dom (\<Gamma>(x \<mapsto> Var ?v))" by blast
-  hence "dom (g\<Gamma>'(x := \<Gamma> x)) = dom \<Gamma>" by auto
-  with T show ?case by blast
-next
-  case (NApp e1 e2)
-  then obtain e\<^sub>1' k t\<^sub>1 t\<^sub>2 vvs' g\<Gamma>' e\<^sub>2' t\<^sub>3 \<Gamma>'' sub where T: "k = ''Arrow'' \<and>
-    typecheck' \<Gamma> vs e1 = Some (e\<^sub>1', Ctor k [t\<^sub>1, t\<^sub>2], vvs', g\<Gamma>') \<and> 
-      typecheck' g\<Gamma>' vvs' e2 = Some (e\<^sub>2', t\<^sub>3, vs', \<Gamma>'') \<and> unify t\<^sub>1 t\<^sub>2 = Some sub \<and> 
-        e' = HApp (hsubst sub e\<^sub>1') (hsubst sub e\<^sub>2') \<and> t = subst sub t\<^sub>2 \<and> 
-          \<Gamma>' = map_option (subst sub) \<circ> \<Gamma>''" 
-    by (auto split: option.splits uexpr.splits list.splits if_splits)
-  with NApp have "dom g\<Gamma>' = dom \<Gamma>" by blast
-  moreover from NApp T have "dom \<Gamma>'' = dom g\<Gamma>'" by blast
-  ultimately have "dom (map_option (subst sub) \<circ> \<Gamma>'') = dom \<Gamma>" by simp
-  with T show ?case by blast
-qed (simp_all split: option.splits)
-
-lemma [simp]: "valid_ty_subst \<Gamma> \<Longrightarrow> typecheck' \<Gamma> vs e = Some (e', t, vs', \<Gamma>') \<Longrightarrow> 
-  valid_ty_subst \<Gamma>' \<and> valid_ty_uexpr t \<and> valid_ty_hexpr e'"
-proof (induction e arbitrary: \<Gamma> vs e' t vs' \<Gamma>')
-  case (NLam x e)
-  let ?v = "fresh vs"
-  from NLam obtain ee' tt g\<Gamma>' t' where T: "g\<Gamma>' x = Some t' \<and> 
-    typecheck' (\<Gamma>(x \<mapsto> Var ?v)) (insert ?v vs) e = Some (ee', tt, vs', g\<Gamma>') \<and> 
-      e' = HLam x t' ee' \<and> t = Ctor ''Arrow'' [t', tt] \<and> \<Gamma>' = (g\<Gamma>'(x := \<Gamma> x))" 
-    by (auto simp add: Let_def split: option.splits prod.splits)
+  from NLam obtain ee' tt where T: "e' = HLam x (Var ?v) ee' \<and> 
+    t = Ctor ''Arrow'' [Var ?v, tt] \<and> 
+      typecheck' (\<Gamma>(x \<mapsto> Var ?v)) (insert ?v vs) e = Some (ee', tt, vs', uni)" 
+    by (auto simp add: Let_def split: option.splits)
   from NLam have "valid_ty_subst (\<Gamma>(x \<mapsto> Var ?v))" by simp
-  with NLam T have X: "valid_ty_subst g\<Gamma>' \<and> valid_ty_uexpr tt \<and> valid_ty_hexpr ee'" by blast
-  with T have "valid_ty_uexpr t'" by auto
-  with NLam X have "valid_ty_subst (g\<Gamma>'(x := \<Gamma> x)) \<and> valid_ty_uexpr (Ctor ''Arrow'' [t', tt]) \<and> 
-    valid_ty_hexpr (HLam x t' ee')" by simp
+  with NLam T have "valid_ty_uexpr tt \<and> valid_ty_hexpr ee'" by blast
+  with NLam have "valid_ty_uexpr (Ctor ''Arrow'' [Var ?v, tt]) \<and> 
+    valid_ty_hexpr (HLam x (Var ?v) ee')" by simp
   with T show ?case by blast
 next
   case (NApp e1 e2)
-  from NApp(4) obtain e\<^sub>1' t\<^sub>1 t\<^sub>2 vvs' g\<Gamma>' e\<^sub>2' t\<^sub>3 g\<Gamma>'' sub where T: "unify t\<^sub>1 t\<^sub>2 = Some sub \<and> 
-    t = subst sub t\<^sub>2 \<and> e' = HApp (hsubst sub e\<^sub>1') (hsubst sub e\<^sub>2') \<and> 
-      \<Gamma>' = map_option (subst sub) \<circ> g\<Gamma>'' \<and> 
-        typecheck' \<Gamma> vs e1 = Some (e\<^sub>1', Ctor ''Arrow'' [t\<^sub>1, t\<^sub>2], vvs', g\<Gamma>') \<and>
-          typecheck' g\<Gamma>' vvs' e2 = Some (e\<^sub>2', t\<^sub>3, vs', g\<Gamma>'')" 
-    by (auto split: option.splits prod.splits uexpr.splits list.splits if_splits)
-  moreover with NApp have "valid_ty_subst g\<Gamma>' \<and> valid_ty_uexpr (Ctor ''Arrow'' [t\<^sub>1, t\<^sub>2]) \<and> 
-    valid_ty_hexpr e\<^sub>1'" by blast
-  moreover with NApp T have "valid_ty_subst g\<Gamma>'' \<and> valid_ty_uexpr t\<^sub>3 \<and> 
-    valid_ty_hexpr e\<^sub>2'" by blast
-  ultimately have "valid_ty_subst g\<Gamma>'' \<and> valid_ty_subst sub \<and> valid_ty_uexpr t\<^sub>2 \<and> 
-    valid_ty_hexpr e\<^sub>1' \<and> valid_ty_hexpr e\<^sub>2'" by auto
-  hence "valid_ty_subst (map_option (subst sub) \<circ> g\<Gamma>'') \<and> valid_ty_uexpr (subst sub t\<^sub>2) \<and> 
-    valid_ty_hexpr (HApp (hsubst sub e\<^sub>1') (hsubst sub e\<^sub>2'))" by simp
-  with T show ?case by blast
+  from NApp(4) obtain e\<^sub>1' t\<^sub>1 vvs' uni\<^sub>1 e\<^sub>2' t\<^sub>3 uni\<^sub>2 where T: "e' = HApp e\<^sub>1' e\<^sub>2' \<and> 
+    typecheck' \<Gamma> vs e1 = Some (e\<^sub>1', Ctor ''Arrow'' [t\<^sub>1, t], vvs', uni\<^sub>1) \<and> 
+      typecheck' \<Gamma> vvs' e2 = Some (e\<^sub>2', t\<^sub>3, vs', uni\<^sub>2) \<and>
+        uni = (t\<^sub>1, t\<^sub>3) # uni\<^sub>1 @ uni\<^sub>2" 
+          by (auto split: option.splits uexpr.splits list.splits if_splits)
+  moreover with NApp have "valid_ty_uexpr (Ctor ''Arrow'' [t\<^sub>1, t]) \<and> valid_ty_hexpr e\<^sub>1'" by blast
+  moreover with NApp T have "valid_ty_uexpr t\<^sub>3 \<and> valid_ty_hexpr e\<^sub>2'" by blast
+  ultimately show ?case by simp
 qed (auto split: option.splits)
 
-lemma [elim]: "valid_ty_subst \<Gamma> \<Longrightarrow> typecheck' \<Gamma> vs e = Some (e', t, vs', \<Gamma>') \<Longrightarrow> valid_ty_uexpr t"
+lemma [elim]: "valid_ty_subst \<Gamma> \<Longrightarrow> typecheck' \<Gamma> vs e = Some (e', t, vs', uni) \<Longrightarrow> 
+    valid_ty_uexpr t"
   by simp
 
-lemma [simp]: "typecheck' \<Gamma> vs e = Some (e', t, vs', \<Gamma>') \<Longrightarrow> valid_ty_subst \<Gamma> \<Longrightarrow> 
-  map_option typeify \<circ> \<Gamma>' \<turnstile>\<^sub>n solidify e' : typeify t"
-proof (induction e arbitrary: \<Gamma> vs e' t vs' \<Gamma>')
+lemma [simp]: "typecheck' \<Gamma> vs e = Some (e', t, vs', uni) \<Longrightarrow> unify' uni = Some sub \<Longrightarrow> 
+    map_option (typeify \<circ> subst sub) \<circ> \<Gamma> \<turnstile>\<^sub>n solidify (hsubst sub e') : typeify (subst sub t)"
+proof (induction e arbitrary: \<Gamma> vs e' t vs' uni sub)
+  case (NVar x)
+  hence T: "\<Gamma> x = Some t \<and> e' = HVar x \<and> vs' = vs \<and> uni = []" by (simp split: option.splits)
+  moreover with NVar have "sub = Map.empty" by simp
+  moreover from T have "map_option (typeify \<circ> subst Map.empty) \<circ> \<Gamma> \<turnstile>\<^sub>n 
+    solidify (hsubst Map.empty (HVar x)) : typeify (subst Map.empty t)" by simp
+  ultimately show ?case by blast
+next
+  case (NConst k)
+  hence "e' = HConst k \<and> t = Ctor ''Base'' [] \<and> vs' = vs \<and> uni = []" by simp
+  hence "map_option (typeify \<circ> subst sub) \<circ> \<Gamma> \<turnstile>\<^sub>n solidify (hsubst sub e') : typeify (subst sub t)" 
+    by simp
+  thus ?case by blast
+next
   case (NLam x e)
   let ?v = "fresh vs"
-  from NLam obtain ee' tt g\<Gamma>' t' where T: "g\<Gamma>' x = Some t' \<and> 
-    typecheck' (\<Gamma>(x \<mapsto> Var ?v)) (insert ?v vs) e = Some (ee', tt, vs', g\<Gamma>') \<and> 
-      e' = HLam x t' ee' \<and> t = Ctor ''Arrow'' [t', tt] \<and> \<Gamma>' = (g\<Gamma>'(x := \<Gamma> x))" 
-    by (auto simp add: Let_def split: option.splits prod.splits)
-  hence X: "g\<Gamma>' = (\<Gamma>'(x \<mapsto> t'))" by auto
-  from NLam have "valid_ty_subst (\<Gamma>(x \<mapsto> Var ?v))" by simp
-  with NLam(1) T have "map_option typeify \<circ> g\<Gamma>' \<turnstile>\<^sub>n solidify ee' : typeify tt" by blast
-  with X have "map_option typeify \<circ> \<Gamma>' \<turnstile>\<^sub>n solidify (HLam x t' ee') : 
-    typeify (Ctor ''Arrow'' [t', tt])" by simp
-  with T show ?case by blast
+  from NLam obtain ee' tt where T: "e' = HLam x (Var ?v) ee' \<and> t = Ctor ''Arrow'' [Var ?v, tt] \<and>
+    typecheck' (\<Gamma>(x \<mapsto> Var ?v)) (insert ?v vs) e = Some (ee', tt, vs', uni)" 
+      by (auto simp add: Let_def split: option.splits)
+  thus ?case 
+  proof (cases "sub ?v")
+    case None
+    from NLam T have "map_option (typeify \<circ> subst sub) \<circ> (\<Gamma>(x \<mapsto> Var ?v)) \<turnstile>\<^sub>n 
+      solidify (hsubst sub ee') : typeify (subst sub tt)" by blast
+    with None have "map_option (typeify \<circ> subst sub) \<circ> \<Gamma> \<turnstile>\<^sub>n 
+      solidify (hsubst sub (HLam x (Var ?v) ee')) : 
+        typeify (subst sub (Ctor ''Arrow'' [Var ?v, tt]))" by simp
+    with T show ?thesis by blast
+  next
+    case (Some t')
+    from NLam T have "map_option (typeify \<circ> subst sub) \<circ> (\<Gamma>(x \<mapsto> Var ?v)) \<turnstile>\<^sub>n 
+      solidify (hsubst sub ee') : typeify (subst sub tt)" by blast
+    with Some have "map_option (typeify \<circ> subst sub) \<circ> \<Gamma> \<turnstile>\<^sub>n 
+      solidify (hsubst sub (HLam x (Var ?v) ee')) : 
+        typeify (subst sub (Ctor ''Arrow'' [Var ?v, tt]))" by simp
+    with T show ?thesis by blast
+  qed
 next
-  case (NApp e1 e2)
-  from NApp(3) obtain e\<^sub>1' t\<^sub>1 t\<^sub>2 vvs' g\<Gamma>' e\<^sub>2' t\<^sub>3 g\<Gamma>'' sub where T: "unify t\<^sub>1 t\<^sub>2 = Some sub \<and> 
-    t = subst sub t\<^sub>2 \<and> e' = HApp (hsubst sub e\<^sub>1') (hsubst sub e\<^sub>2') \<and> 
-      \<Gamma>' = map_option (subst sub) \<circ> g\<Gamma>'' \<and> 
-        typecheck' \<Gamma> vs e1 = Some (e\<^sub>1', Ctor ''Arrow'' [t\<^sub>1, t\<^sub>2], vvs', g\<Gamma>') \<and>
-          typecheck' g\<Gamma>' vvs' e2 = Some (e\<^sub>2', t\<^sub>3, vs', g\<Gamma>'')" 
-    by (auto split: option.splits prod.splits uexpr.splits list.splits if_splits)
-  with NApp(4) have X: "valid_ty_subst g\<Gamma>' \<and> valid_ty_uexpr (Ctor ''Arrow'' [t\<^sub>1, t\<^sub>2]) \<and> 
-    valid_ty_hexpr e\<^sub>1'" by fastforce
-  with NApp T have Z: "map_option typeify \<circ> g\<Gamma>'' \<turnstile>\<^sub>n solidify e\<^sub>2' : typeify t\<^sub>3" by blast
-  from T X have Y: "valid_ty_subst g\<Gamma>'' \<and> valid_ty_uexpr t\<^sub>3 \<and> valid_ty_hexpr e\<^sub>2'" by fastforce
+  case (NApp e\<^sub>1 e\<^sub>2)
+  then obtain e\<^sub>1' t\<^sub>1 xvs' uni\<^sub>1 e\<^sub>2' t\<^sub>3 uni\<^sub>2 where T: "e' = HApp e\<^sub>1' e\<^sub>2' \<and> uni = (t\<^sub>1, t\<^sub>3) # uni\<^sub>1 @ uni\<^sub>2 \<and>
+    typecheck' \<Gamma> vs e\<^sub>1 = Some (e\<^sub>1', Ctor ''Arrow'' [t\<^sub>1, t], xvs', uni\<^sub>1) \<and>
+      typecheck' \<Gamma> xvs' e\<^sub>2 = Some (e\<^sub>2', t\<^sub>3, vs', uni\<^sub>2)" 
+        by (auto split: option.splits if_splits uexpr.splits list.splits)
 
 
-  from NApp T have "map_option typeify \<circ> g\<Gamma>' \<turnstile>\<^sub>n solidify e\<^sub>1' : typeify (Ctor ''Arrow'' [t\<^sub>1, t\<^sub>2])" by blast
-  hence "map_option typeify \<circ> g\<Gamma>' \<turnstile>\<^sub>n solidify e\<^sub>1' : Arrow (typeify t\<^sub>1) (typeify t\<^sub>2)" by simp
+  from NApp T have "unify' uni\<^sub>1 = Some sub\<^sub>1 \<Longrightarrow> 
+    map_option (typeify \<circ> subst sub\<^sub>1) \<circ> \<Gamma> \<turnstile>\<^sub>n solidify (hsubst sub\<^sub>1 e\<^sub>1') : typeify (subst sub\<^sub>1 (Ctor ''Arrow'' [t\<^sub>1, t]))" 
+      by blast
+  from NApp T have "unify' uni\<^sub>2 = Some sub\<^sub>2 \<Longrightarrow> 
+    map_option (typeify \<circ> subst sub\<^sub>2) \<circ> \<Gamma> \<turnstile>\<^sub>n solidify (hsubst sub\<^sub>2 e\<^sub>2') : typeify (subst sub\<^sub>2 t\<^sub>3)" by blast
+
+
+  from NApp have "unify' uni = Some sub" by simp
 
 
 
 
-  have "map_option typeify \<circ> g\<Gamma>'' \<turnstile>\<^sub>n solidify e\<^sub>1' : Arrow (typeify t\<^sub>3) (typeify t\<^sub>2)" by simp
-  with Z have "map_option typeify \<circ> g\<Gamma>'' \<turnstile>\<^sub>n TApp (solidify e\<^sub>1') (solidify e\<^sub>2') : typeify t\<^sub>2" by simp
-  hence "map_option (tsubsts sub) \<circ> (map_option typeify \<circ> g\<Gamma>'') \<turnstile>\<^sub>n 
-    tsubstt sub (TApp (solidify e\<^sub>1') (solidify e\<^sub>2')) : tsubsts sub (typeify t\<^sub>2)" 
-      by (metis tc_tsubstt)
-  with X Y have "map_option typeify \<circ> (map_option (subst sub) \<circ> g\<Gamma>'') \<turnstile>\<^sub>n 
-    solidify (HApp (hsubst sub e\<^sub>1') (hsubst sub e\<^sub>2')) : typeify (subst sub t\<^sub>2)" by simp
+  have X: "map_option (typeify \<circ> subst sub) \<circ> \<Gamma> \<turnstile>\<^sub>n solidify (hsubst sub e\<^sub>1') : Arrow xt\<^sub>1 (typeify (subst sub t))" by simp
+
+
+  have "map_option (typeify \<circ> subst sub) \<circ> \<Gamma> \<turnstile>\<^sub>n solidify (hsubst sub e\<^sub>2') : xt\<^sub>1" by simp
+  with X have "map_option (typeify \<circ> subst sub) \<circ> \<Gamma> \<turnstile>\<^sub>n solidify (hsubst sub (HApp e\<^sub>1' e\<^sub>2')) : 
+    typeify (subst sub t)" by simp
   with T show ?case by blast
-qed (auto split: option.splits)
+qed
 
 lemma [simp]: "typecheck e = Some (e\<^sub>t, t) \<Longrightarrow> Map.empty \<turnstile>\<^sub>n e\<^sub>t : t"
 proof -
   assume "typecheck e = Some (e\<^sub>t, t)"
-  then obtain e' tt vs \<Gamma> where T: "typecheck' Map.empty {} e = Some (e', tt, vs, \<Gamma>) \<and> 
-    e\<^sub>t = solidify e' \<and> t = typeify tt" by (auto split: option.splits)
-  moreover hence "map_option typeify \<circ> \<Gamma> \<turnstile>\<^sub>n solidify e' : typeify tt" by auto
-  moreover from T have "dom \<Gamma> = dom Map.empty" by force
-  ultimately show "Map.empty \<turnstile>\<^sub>n e\<^sub>t : t" by simp
+  then obtain e' tt vs \<Gamma> uni sub where T: "typecheck' Map.empty {} e = Some (e', tt, vs, \<Gamma>, uni) \<and>
+    unify' uni = Some sub \<and> e\<^sub>t = solidify (hsubst sub e') \<and> t = typeify (subst sub tt)" 
+      by (auto split: option.splits)
+
+
+
+  have "Map.empty \<turnstile>\<^sub>n solidify (hsubst sub e') : typeify (subst sub tt)" by simp
+  with T show "Map.empty \<turnstile>\<^sub>n e\<^sub>t : t" by simp
 qed
 
 lemma erase_solidify [simp]: "valid_ty_subst \<Gamma> \<Longrightarrow> typecheck' \<Gamma> vs e = Some (e', t, vs', \<Gamma>') \<Longrightarrow> 
@@ -297,60 +317,56 @@ proof -
   with T show ?thesis by simp
 qed
 
-lemma [dest]: "NVar x = erase e\<^sub>t \<Longrightarrow> e\<^sub>t = TVar x"
+lemma [dest]: "erase e\<^sub>t = NVar x \<Longrightarrow> e\<^sub>t = TVar x"
   by (induction e\<^sub>t) simp_all
 
-lemma [dest]: "NLam x e = erase e\<^sub>t \<Longrightarrow> \<exists>t e\<^sub>t'. e\<^sub>t = TLam x t e\<^sub>t' \<and> e = erase e\<^sub>t'"
+lemma [dest]: "erase e\<^sub>t = NLam x e \<Longrightarrow> \<exists>t e\<^sub>t'. e\<^sub>t = TLam x t e\<^sub>t' \<and> e = erase e\<^sub>t'"
   by (induction e\<^sub>t) simp_all
 
-lemma [simp]: "typecheck' \<Gamma> vs e = None \<Longrightarrow> \<nexists>e\<^sub>t t. (map_option typeify \<circ> \<Gamma> \<turnstile>\<^sub>n e\<^sub>t : t) \<and> e = erase e\<^sub>t"
-proof (induction e arbitrary: \<Gamma> vs)
+lemma typecheck_fails' [simp]: "typecheck' \<Gamma> vs e = None \<Longrightarrow> map_option typeify \<circ> \<Gamma> \<turnstile>\<^sub>n e\<^sub>t : t \<Longrightarrow> 
+  erase e\<^sub>t = e \<Longrightarrow> False"
+proof (induction e arbitrary: \<Gamma> vs e\<^sub>t t)
   case (NVar x)
-  hence X: "\<Gamma> x = None" by (simp split: option.splits)
-  have "\<And>e\<^sub>t. NVar x = erase e\<^sub>t \<Longrightarrow> \<nexists>t. map_option typeify \<circ> \<Gamma> \<turnstile>\<^sub>n e\<^sub>t : t"
-  proof 
-    fix e\<^sub>t
-    assume "NVar x = erase e\<^sub>t" 
-    hence "e\<^sub>t = TVar x" by blast
-    moreover assume "\<exists>t. map_option typeify \<circ> \<Gamma> \<turnstile>\<^sub>n e\<^sub>t : t"
-    ultimately obtain t where "(map_option typeify \<circ> \<Gamma>) x = Some t" by blast
-    with X show False by simp
-  qed
-  thus ?case by blast
+  hence "\<Gamma> x = None" by (simp split: option.splits)
+  moreover from NVar have "(map_option typeify \<circ> \<Gamma>) x = Some t" by blast
+  ultimately show ?case by simp
 next
   case (NLam x e)
   let ?v = "fresh vs"
-  have "\<And>e\<^sub>t. NLam x e = erase e\<^sub>t \<Longrightarrow> \<nexists>t. map_option typeify \<circ> \<Gamma> \<turnstile>\<^sub>n e\<^sub>t : t"
-  proof
-    fix e\<^sub>t
-    assume "NLam x e = erase e\<^sub>t" 
-    then obtain t\<^sub>1 e\<^sub>t' where E: "e\<^sub>t = TLam x t\<^sub>1 e\<^sub>t' \<and> e = erase e\<^sub>t'" by blast
-    moreover assume "\<exists>t. map_option typeify \<circ> \<Gamma> \<turnstile>\<^sub>n e\<^sub>t : t"
-    ultimately obtain t\<^sub>2 where "(map_option typeify \<circ> \<Gamma>)(x \<mapsto> t\<^sub>1) \<turnstile>\<^sub>n e\<^sub>t' : t\<^sub>2" by blast
-    show False
-    proof (cases "typecheck' (\<Gamma>(x \<mapsto> Var ?v)) (insert ?v vs) e")
-      case None
-      with NLam E have "\<And>t. \<not> map_option typeify \<circ> (\<Gamma>(x \<mapsto> Var ?v)) \<turnstile>\<^sub>n e\<^sub>t' : t" by blast
-    
-    
-      show False by blast
-    next
-      case (Some a)
-      with NLam have "\<exists>e' t vs' \<Gamma>'. typecheck' (\<Gamma>(x \<mapsto> Var ?v)) (insert ?v vs) e = Some (e', t, vs', \<Gamma>') \<and> \<Gamma>' x = None" 
+  show ?case
+  proof (cases "typecheck' (\<Gamma>(x \<mapsto> Var ?v)) (insert ?v vs) e")
+    case None
+
+    from NLam obtain t\<^sub>1 e\<^sub>t' where E: "e\<^sub>t = TLam x t\<^sub>1 e\<^sub>t' \<and> e = erase e\<^sub>t'" by blast
+    from NLam E obtain t\<^sub>2 where "((map_option typeify \<circ> \<Gamma>)(x \<mapsto> t\<^sub>1) \<turnstile>\<^sub>n e\<^sub>t' : t\<^sub>2) \<and> t = Arrow t\<^sub>1 t\<^sub>2" 
+      by blast
+
+
+
+    have "(map_option typeify \<circ> \<Gamma>)(x \<mapsto> TyVar ?v) \<turnstile>\<^sub>n e\<^sub>t' : xt" by simp
+    hence "map_option typeify \<circ> (\<Gamma>(x \<mapsto> Var ?v)) \<turnstile>\<^sub>n e\<^sub>t' : xt" by simp
+    with NLam E None show ?thesis by blast
+  next
+    case (Some a)
+    with NLam obtain e' t' vs' \<Gamma>' where G: "\<Gamma>' x = None \<and> 
+      typecheck' (\<Gamma>(x \<mapsto> Var ?v)) (insert ?v vs) e = Some (e', t', vs', \<Gamma>')" 
         by (auto simp add: Let_def split: option.splits prod.splits)
-    
-    
-      show False by blast
-    qed
+    hence "dom \<Gamma>' = dom (\<Gamma>(x \<mapsto> Var ?v))" by force
+    with G show ?thesis by auto
   qed
-  thus ?case by blast
 next
   case (NApp e1 e2)
-  then show ?case by simp
+  thus ?case by simp
 qed simp_all
 
 lemma typecheck_fails [simp]: "typecheck e = None \<Longrightarrow> \<nexists>e\<^sub>t t. (Map.empty \<turnstile>\<^sub>n e\<^sub>t : t) \<and> e = erase e\<^sub>t"
-  by simp
+proof 
+  assume "typecheck e = None"
+  hence X: "typecheck' Map.empty {} e = None" by (simp split: option.splits prod.splits)
+  assume "\<exists>e\<^sub>t t. (Map.empty \<turnstile>\<^sub>n e\<^sub>t : t) \<and> e = erase e\<^sub>t"
+  then obtain e\<^sub>t t where "(map_option typeify \<circ> Map.empty \<turnstile>\<^sub>n e\<^sub>t : t) \<and> e = erase e\<^sub>t" by fastforce
+  with X show "False" by (metis typecheck_fails')
+qed
 
 lemma [simp]: "valn (erase e) = valt e"
   by (induction e) simp_all
